Models/Trace.thy
@@ -1,5 +1,5 @@
 theory Trace
-  imports Stutter_Language Algebra
+  imports Aczel Mumble_Language Rely_Guarantee Algebra
 begin
 
 no_notation shuffle (infixl "\<parallel>" 75)
@@ -21,7 +21,7 @@ begin
 
   lift_definition zero_trace :: "'a trace" is "{}" done
 
-  lift_definition one_trace :: "'a trace" is "{LNil}\<^sup>\<dagger>" done
+  lift_definition one_trace :: "'a trace" is "{LNil}" done
 
   lift_definition times_trace :: "'a trace \<Rightarrow> 'a trace \<Rightarrow> 'a trace" is "\<lambda>X Y. l_prod X\<^sup>\<dagger> Y\<^sup>\<dagger>"
     by simp
@@ -41,15 +41,15 @@ begin
     show "(x + y) \<cdot> z = x \<cdot> z + y \<cdot> z"
       by transfer simp
     show "1 \<cdot> x = x"
-      by transfer (simp only: Stutter_idem Stutter_l_prod l_prod_one)
+      by transfer simp
     show "x \<cdot> 1 = x"
-      by transfer (simp only: Stutter_idem Stutter_l_prod l_prod_one)
+      by transfer simp
     show "0 + x = x"
       by transfer simp
     show "0 \<cdot> x = 0"
       by transfer simp
     show "(x \<le> y) = (x + y = y)"
-      by transfer (metis Stutter_union par.add_commute sup.order_iff)
+      by transfer (metis Mumble_union par.add_commute sup.order_iff)
     show "(x < y) = (x \<le> y \<and> x \<noteq> y)"
       by transfer (metis par.less_def)
     show "x + x = x"
@@ -66,40 +66,68 @@ lift_definition Aczel_trace :: "'a trace \<Rightarrow> 'a trace" ("\<pi>") is "\
 (* \<pi> is an interior operator *)
 
 lemma proj_coextensive [intro!]: "\<pi> x \<le> x"
-  by transfer (metis Aczel_coextensive Stutter_idem Stutter_iso)
+  by transfer (metis Aczel_coextensive Mumble_idem Mumble_iso)
 
 lemma proj_iso [intro]: "x \<le> y \<Longrightarrow> \<pi> x \<le> \<pi> y"
-  by transfer (metis Aczel_iso Stutter_iso)
+  by transfer (metis Aczel_iso Mumble_iso)
+
+lemma [simp]: "(Aczel x\<^sup>\<dagger>)\<^sup>\<dagger> = (Aczel x)\<^sup>\<dagger>"
+  by (auto simp add: Aczel_def Con_def Mumble_def) (metis mumble_preserves_consistent mumble_trans)
 
 lemma proj_idem [simp]: "\<pi> (\<pi> x) = \<pi> x"
-  by transfer (metis Aczel_idem Stutter_proj)
+  by transfer simp
 
-lemma proj_plus [simp]: "\<pi> (x + y) = \<pi> x + \<pi> y"
-  by transfer (metis Aczel_union Stutter_union)
+lemma proj_plus [simp]: "\<pi> x + \<pi> y = \<pi> (x + y)"
+  by transfer (metis Aczel_union Mumble_union)
 
 lemma proj_mult [simp]: "\<pi> (\<pi> x \<cdot> \<pi> y) = \<pi> (x \<cdot> y)"
-  by transfer (metis Aczel_l_prod Stutter_l_prod Stutter_proj)
+  by transfer simp
 
 lemma proj_mult2 [simp]: "\<pi> (\<pi> x \<cdot> y) = \<pi> (x \<cdot> y)"
-  by transfer (metis Aczel_idem Aczel_l_prod Stutter_l_prod Stutter_proj)
+  by transfer (metis Aczel_trace.abs_eq proj_idem proj_mult times_trace.abs_eq trace.abs_eq_iff)
 
 lemma proj_mult3 [simp]: "\<pi> (x \<cdot> \<pi> y) = \<pi> (x \<cdot> y)"
   by (metis proj_mult proj_mult2)
 
 (* Tests *)
 
-no_notation test ("\<langle>_\<rangle>" [0] 1000)
+no_notation atomic ("\<langle>_\<rangle>" [0] 1000)
 
-lift_definition test_trace :: "'a set \<Rightarrow> 'a trace" ("\<langle>_\<rangle>" [0] 1000) is "\<lambda>S. test S" by simp
+lift_definition atomic_trace :: "'a rel \<Rightarrow> 'a trace" ("\<langle>_\<rangle>" [0] 1000) is "\<lambda>S. atomic S" by simp
 
-lemma "\<langle>X\<rangle> \<le> 1"
-  by transfer (simp, intro Stutter_iso test_iso subset_UNIV)
+definition test :: "'a set \<Rightarrow> 'a trace" where
+  "test X = \<langle>Id_on X\<rangle>"
 
-lemma "\<pi> (\<langle>X\<rangle> \<cdot> \<langle>Y\<rangle>) = \<pi> (\<langle>X \<inter> Y\<rangle>)"
-  by transfer (metis Aczel_mult_def Stutter_l_prod Stutter_proj test_l_prod)
+lemma atomic_test: "atomic (Id_on X) = {LCons (\<sigma>, \<sigma>') LNil |\<sigma> \<sigma>'. \<sigma> \<in> X \<and> \<sigma> = \<sigma>'}"
+  sorry
+
+lemma "\<pi> (test (X \<inter> Y)) \<le> \<pi> (test X \<cdot> test Y)"
+  apply (simp only: test_def)
+  apply transfer
+  apply (simp add: atomic_test)
+  apply (subst fin_l_prod)
+  apply (force simp add: FIN_def)
+  apply (auto simp add: Aczel_def Con_def Mumble_def)
+  apply (rule_tac x = "mumble (LCons (\<sigma>, \<sigma>) (LCons (\<sigma>, \<sigma>) LNil))" in exI)
+  apply (intro conjI)
+  apply (rule_tac x = "LCons (\<sigma>, \<sigma>) (LCons (\<sigma>, \<sigma>) LNil)" in exI)
+  apply (metis LCons_lappend_LNil inconsistent_mumble lappend_code(1) lfinite.simps)
+  by (metis lappend_code(1) mumble.mumble mumble.self mumble_trans)
+
+lemma [dest!]: "ys \<frown> LCons z (LCons z' zs) = LCons x LNil \<Longrightarrow> False"
+  apply (cases "lfinite ys")
+  apply (rotate_tac 1)
+  apply (induct ys rule: lfinite.induct)
+  by (simp_all add: lappend_inf)
+
+lemma [dest!]: "xs \<in> mumble (LCons x LNil) \<Longrightarrow> xs = LCons x LNil"
+  by (induct xs rule: mumble.induct) auto
+
+lemma Mumble_atomic [simp]: "(atomic X)\<^sup>\<dagger> = atomic X"
+  by (auto simp add: Mumble_def atomic_def image_def)
 
 lemma "\<langle>X\<rangle> + \<langle>Y\<rangle> = \<langle>X \<union> Y\<rangle>"
-  by transfer (metis test_union)
+  by transfer (metis Mumble_atomic atomic_def image_Un)
 
 (* traces form a dioid w.r.t. parallel composition *)
 
@@ -116,9 +144,9 @@ begin
     show "x \<parallel> y = y \<parallel> x"
       by transfer (metis shuffle_comm)
     show "x \<parallel> (y + z) = x \<parallel> y + x \<parallel> z"
-      by transfer (metis Stutter_union par.distrib_left)
+      by transfer (metis Mumble_union par.distrib_left)
     show "1 \<parallel> x = x"
-      by transfer (metis Stutter_shuffle_left par.mult.right_neutral shuffle_comm)
+      by transfer (metis Mumble_shuffle_left par.mult.right_neutral shuffle_comm)
     show "0 \<parallel> x = 0"
       by transfer simp
   qed
@@ -152,13 +180,95 @@ begin
   qed
 end
 
+lift_definition stuttering :: "'a trace" is stutter done
+
 lemma join_is_plus [simp]:
   fixes x y :: "'a trace"
   shows "x \<squnion> y = x + y"
   by transfer simp
 
 instance trace :: (type) distrib_lattice
-  by (default, transfer, simp, metis Stutter_idem Stutter_meet Stutter_union Un_Int_distrib)
+  by (default, transfer, simp, metis Mumble_idem Mumble_meet Mumble_union Un_Int_distrib)
+
+no_notation Language.star ("_\<^sup>\<star>" [101] 100)
+
+instantiation trace :: (type) left_kleene_algebra
+begin
+
+  lift_definition star_trace :: "'a trace \<Rightarrow> 'a trace" is "\<lambda>x. Language.star x\<^sup>\<dagger>"
+    by simp
+
+  instance
+  proof
+    fix x y z :: "'a trace"
+    show "1 + x \<cdot> x\<^sup>\<star> \<le> x\<^sup>\<star>"
+      by transfer (metis Mumble_l_prod Mumble_star Mumble_union par.less_eq_def seq.add_idem' seq.star_unfoldl_eq)
+    show "z + x \<cdot> y \<le> y \<longrightarrow> x\<^sup>\<star> \<cdot> z \<le> y"
+      by transfer (metis Mumble_ext Mumble_idem Mumble_iso Mumble_l_prod order.trans seq.star_inductl)
+  qed
+end
+
+lemma [simp]: "set_rel (llist_all2 (prod_rel op = op =)) x y \<longleftrightarrow> x = y"
+  by (auto simp add: prod_rel_eq set_rel_def)
+
+lemma [simp]: "pcr_trace op = x y \<longleftrightarrow> abs_trace x = y"
+  by (simp add: pcr_trace_def OO_def cr_trace_def)
+
+lemma [simp]: "abs_trace X = Abs_trace {Y. X\<^sup>\<dagger> = Y\<^sup>\<dagger>}"
+  apply (auto simp add: abs_trace_def)
+  apply (subst quot_type.abs_def[of _ _ Rep_trace])
+  apply (auto simp add: quot_type_def)
+  apply (metis equivp_implies_part_equivp trace_equivp)
+  defer
+  apply (metis Rep_trace_inverse)
+  apply (erule rev_mp)+
+  apply (subst Abs_trace_inverse)
+  apply auto
+  apply (erule rev_mp)+
+  apply (subst Abs_trace_inverse)
+  apply auto
+  apply (subst Abs_trace_inverse)
+  apply auto
+  apply (metis Rep_trace_inject)
+  apply (insert Rep_trace)
+  by auto
+
+lemma [transfer_rule]: "(pcr_trace op = ===> set_rel (pcr_trace op =) ===> op =) (\<lambda>X Y. X\<^sup>\<dagger> \<in> Mumble ` Y) op \<in>"
+  apply (auto simp add: fun_rel_def set_rel_def image_def)
+  apply (erule_tac x = "Abs_trace {Y. x\<^sup>\<dagger> = Y\<^sup>\<dagger>}" in ballE)
+  apply auto
+  apply (rule_tac x = xb in bexI)
+  apply simp_all
+  apply (erule rev_mp)+
+  apply (subst Abs_trace_inject)
+  by auto
+
+lemma [transfer_rule]: "(op = ===> pcr_trace op = ===> op =) (\<lambda>x y. x = Abs_trace {Y. y\<^sup>\<dagger> = Y\<^sup>\<dagger>}) op ="
+  by (auto simp add: fun_rel_def)
+
+instantiation trace :: (type) rely_guarantee_trioid
+begin
+
+  lift_definition RG_trace :: "'a trace set" is "{x. \<exists>R. x = Language.star (atomic R)}" done
+
+  lift_definition \<C>_trace :: "'a trace" is Aczel.Con done
+
+  instance
+  proof
+    fix r s x y :: "'a trace"
+    show "(1::'a trace) \<in> RG"
+      by transfer (auto intro: exI[of _ "{LNil}"] exI[of _ "{}"] simp add: image_def)
+
+
+
+lemma "\<pi> (test X \<cdot> test Y \<parallel> stuttering) = \<pi> (test (X \<inter> Y) \<parallel> stuttering)"
+  sorry
+
+definition proj_eq :: "'a trace \<Rightarrow> 'a trace \<Rightarrow> bool" (infix "=\<^sub>\<pi>" 55) where
+  "x =\<^sub>\<pi> y \<equiv> \<pi> x = \<pi> y"
+
+lemma proj_eq_trans [trans]: "x =\<^sub>\<pi> y \<Longrightarrow> y =\<^sub>\<pi> z \<Longrightarrow> x =\<^sub>\<pi> z"
+  by (simp add: proj_eq_def)
 
 no_notation Aczel_mult (infixl "\<otimes>" 75)
 
@@ -175,7 +285,7 @@ lemma pmult_oner [simp]: "x \<otimes> 1 = \<pi> x"
   by (metis mult_oner pmult_def)
 
 lemma proj_zero [simp]: "\<pi> 0 = 0"
-  by transfer (simp add: Aczel_def)
+  by transfer simp
 
 lemma pmult_zero [simp]: "0 \<otimes> x = 0"
   by (simp add: pmult_def)
@@ -193,9 +303,6 @@ proof
     by (metis add_idem)
 qed
 
-abbreviation proj_eq :: "'a trace \<Rightarrow> 'a trace \<Rightarrow> bool" (infixl "=\<^sub>\<pi>" 55) where
-  "x =\<^sub>\<pi> y \<equiv> (\<pi> x = \<pi> y)"
-
 definition proj_leq :: "'a trace \<Rightarrow> 'a trace \<Rightarrow> bool" (infixl "\<le>\<^sub>\<pi>" 55) where
   "x \<le>\<^sub>\<pi> y \<equiv> (\<pi> x \<le> \<pi> y)"
 
@@ -208,16 +315,16 @@ lemma proj_leq_trans2 [trans]: "x \<le> y \<Longrightarrow> y \<le>\<^sub>\<pi> 
 lemma proj_leq_trans3 [trans]: "x \<le>\<^sub>\<pi> y \<Longrightarrow> y \<le> z \<Longrightarrow> x \<le>\<^sub>\<pi> z"
   by (metis proj_iso proj_leq_def proj_leq_trans)
 
-find_theorems Aczel "op \<inter>"
-find_theorems Stutter "op \<inter>"
+lemma proj_leq_trans4 [trans]: "x \<le>\<^sub>\<pi> y \<Longrightarrow> y =\<^sub>\<pi> z \<Longrightarrow> x \<le>\<^sub>\<pi> z"
+  by (auto simp add: proj_leq_def proj_eq_def)
 
-lemma Stutter_Con: "(X \<inter> Con)\<^sup>\<dagger> = (X \<inter> Con\<^sup>\<dagger>)\<^sup>\<dagger>"EC
-  sorry
+lemma proj_leq_trans5 [trans]: "x =\<^sub>\<pi> y \<Longrightarrow> y \<le>\<^sub>\<pi> z \<Longrightarrow> x \<le>\<^sub>\<pi> z"
+  by (auto simp add: proj_leq_def proj_eq_def)
 
 lemma proj_meet [simp]: "\<pi> x \<sqinter> \<pi> y = \<pi> (x \<sqinter> y)"
   apply transfer
   apply (simp add: Aczel_def)
-  by (metis Aczel_def Int_assoc Stutter_Con Stutter_meet inf_commute inf_left_idem)
+  by (metis Aczel_def Int_assoc Mumble_Con Mumble_meet inf_commute inf_left_idem)
 
 lemma proj_leq_meet [simp]: "\<pi> x \<sqinter> \<pi> y \<le>\<^sub>\<pi> x \<sqinter> y"
   by (metis inf_mono proj_coextensive proj_iso proj_leq_def)
